src/ocaml/our.ml
@@ -1,5 +1,10 @@
 let string_of_chars chars = chars|>List.map (String.make 1)|>String.concat ""
 
+type any_t
+
+let any_ref = ref ((Obj.magic 1):any_t)
+
+
 open Gen_isa
   
 module Util : sig
@@ -7,6 +12,7 @@ module Util : sig
   val split_at : Arith.nat -> 'a list -> 'a list * 'a list
   val rev_apply : 'a -> ('a -> 'b) -> 'b
   val split_at_3 : Arith.nat -> 'a list -> 'a list * ('a * 'a list)
+  val assert_true : 'a -> bool -> bool
 end = struct
 
 let rec failwitha x = x|>string_of_chars|>failwith;;
@@ -19,6 +25,11 @@ let rec split_at_3
   n xs =
     (List.take n xs,
       (List.nth xs n, List.drop (Arith.plus_nat n Arith.one_nat) xs));;
+
+let rec assert_true arg b = (
+  let _ = any_ref := ((Obj.magic arg):any_t) in
+  if b then b else failwith "assert_true")
+;;
 
 
 end;;
@@ -243,19 +254,20 @@ let rec wf_size_1
 
 let rec wf_size
   ms t0 =
-    (match ms with None -> forall_subtrees wf_size_1 t0
-      | Some m ->
-        let min = get_min_size (m, t0) in
-        (match t0
-          with Node (l, cs) ->
-            let n = List.size_list l in
-            Arith.less_eq_nat min n &&
-              (Arith.less_eq_nat n Constants.max_node_keys &&
-                List.pred_list (forall_subtrees wf_size_1) cs)
-          | Leaf xs ->
-            let n = List.size_list xs in
-            Arith.less_eq_nat min n &&
-              Arith.less_eq_nat n Constants.max_leaf_size));;
+    Util.assert_true (ms, t0)
+      (match ms with None -> forall_subtrees wf_size_1 t0
+        | Some m ->
+          let min = get_min_size (m, t0) in
+          (match t0
+            with Node (l, cs) ->
+              let n = List.size_list l in
+              Arith.less_eq_nat min n &&
+                (Arith.less_eq_nat n Constants.max_node_keys &&
+                  List.pred_list (forall_subtrees wf_size_1) cs)
+            | Leaf xs ->
+              let n = List.size_list xs in
+              Arith.less_eq_nat min n &&
+                Arith.less_eq_nat n Constants.max_leaf_size));;
 
 let rec balanced_1
   t0 = (match t0
@@ -268,7 +280,7 @@ let rec balanced_1
                cs
          | Leaf _ -> true);;
 
-let rec balanced t = forall_subtrees balanced_1 t;;
+let rec balanced t = Util.assert_true t (forall_subtrees balanced_1 t);;
 
 let rec wf_ks_rs_1
   t0 = (match t0
@@ -277,7 +289,7 @@ let rec wf_ks_rs_1
              (List.size_list cs)
          | Leaf _ -> true);;
 
-let rec wf_ks_rs t0 = forall_subtrees wf_ks_rs_1 t0;;
+let rec wf_ks_rs t0 = Util.assert_true t0 (forall_subtrees wf_ks_rs_1 t0);;
 
 let rec dest_Leaf
   = function Leaf kvs -> kvs
@@ -311,7 +323,7 @@ let rec tss_to_keys
 let rec keys_ordered_1
   t0 = Util.rev_apply (Util.rev_apply t0 keys_1) Key_value.ordered_key_list;;
 
-let rec keys_ordered t = forall_subtrees keys_ordered_1 t;;
+let rec keys_ordered t = Util.assert_true t (forall_subtrees keys_ordered_1 t);;
 
 let rec tree_to_keys
   t = Util.rev_apply
@@ -357,17 +369,19 @@ let rec keys_consistent_1
              (subtree_indexes (ks, rs))
          | Leaf _ -> true);;
 
-let rec keys_consistent t = forall_subtrees keys_consistent_1 t;;
+let rec keys_consistent
+  t = Util.assert_true t (forall_subtrees keys_consistent_1 t);;
 
 let rec wellformed_tree
   ms t0 =
-    let b1 = wf_size ms t0 in
-    let b2 = wf_ks_rs t0 in
-    let b3 = balanced t0 in
-    let b4 = keys_consistent t0 in
-    let b5 = keys_ordered t0 in
-    let wf = b1 && (b2 && (b3 && (b4 && b5))) in
-    wf;;
+    Util.assert_true (ms, t0)
+      (let b1 = wf_size ms t0 in
+       let b2 = wf_ks_rs t0 in
+       let b3 = balanced t0 in
+       let b4 = keys_consistent t0 in
+       let b5 = keys_ordered t0 in
+       let wf = b1 && (b2 && (b3 && (b4 && b5))) in
+       wf);;
 
 
 end;;
@@ -377,7 +391,7 @@ module Tree_stack : sig
   type ('a, 'b) core_t_ext =
     Core_t_ext of
       Key_value_types.key * (Tree.tree list) list * Key_value_types.key option *
-        'a * Key_value_types.key option * (Tree.tree list) list * 'b
+        'a * Key_value_types.key option * (Tree.tree list) list * 'b[@@deriving yojson]
   val equal_core_t_exta :
     'a HOL.equal -> 'b HOL.equal ->
       ('a, 'b) core_t_ext -> ('a, 'b) core_t_ext -> bool
@@ -412,7 +426,7 @@ end = struct
 type ('a, 'b) core_t_ext =
   Core_t_ext of
     Key_value_types.key * (Tree.tree list) list * Key_value_types.key option *
-      'a * Key_value_types.key option * (Tree.tree list) list * 'b;;
+      'a * Key_value_types.key option * (Tree.tree list) list * 'b[@@deriving yojson];;
 
 let rec equal_core_t_exta _A _B
   (Core_t_ext (f_ka, f_tss1a, f_kla, f_ta, f_kua, f_tss2a, morea))
@@ -452,15 +466,17 @@ let rec dest_core
 
 let rec wf_core
   t_keys x =
-    let (k, (tss1, (kl, (_, (ku, tss2))))) = Util.rev_apply x dest_core in
-    Key_value.check_keys_2 (Util.rev_apply tss1 Tree.tss_to_keys) kl
-      (Set.insert Key_value_types.equal_key k t_keys) ku
-      (Util.rev_apply tss2 Tree.tss_to_keys);;
+    Util.assert_true (t_keys, x)
+      (let (k, (tss1, (kl, (_, (ku, tss2))))) = Util.rev_apply x dest_core in
+       Key_value.check_keys_2 (Util.rev_apply tss1 Tree.tss_to_keys) kl
+         (Set.insert Key_value_types.equal_key k t_keys) ku
+         (Util.rev_apply tss2 Tree.tss_to_keys));;
 
 let rec wf_nf
   ms f =
-    let (ks, ts) = Util.rev_apply f f_t in
-    wf_core (Util.rev_apply (Tree.Node (ks, ts)) Tree.tree_to_keys) f;;
+    Util.assert_true (ms, f)
+      (let (ks, ts) = Util.rev_apply f f_t in
+       wf_core (Util.rev_apply (Tree.Node (ks, ts)) Tree.tree_to_keys) f);;
 
 let rec with_t
   f x = let (k, (tss1, (kl, (t, (ku, tss2))))) = Util.rev_apply x dest_core in
@@ -529,19 +545,20 @@ let rec mk_next_frame
         | Tree.Leaf _ -> None);;
 
 let rec wellformed_ts
-  xs = (match xs with [] -> true
-         | c :: xsa ->
-           wf_nf (ts_to_ms xsa) c &&
-             (wellformed_ts xsa &&
-               (match xsa with [] -> true
-                 | p :: _ ->
-                   Option.equal_option
-                     (equal_core_t_ext
-                       (Product_Type.equal_prod
-                         (List.equal_list Key_value_types.equal_key)
-                         (List.equal_list Tree.equal_Tree))
-                       Product_Type.equal_unit)
-                     (mk_next_frame p) (Some c))));;
+  xs = Util.assert_true xs
+         (match xs with [] -> true
+           | c :: xsa ->
+             wf_nf (ts_to_ms xsa) c &&
+               (wellformed_ts xsa &&
+                 (match xsa with [] -> true
+                   | p :: _ ->
+                     Option.equal_option
+                       (equal_core_t_ext
+                         (Product_Type.equal_prod
+                           (List.equal_list Key_value_types.equal_key)
+                           (List.equal_list Tree.equal_Tree))
+                         Product_Type.equal_unit)
+                       (mk_next_frame p) (Some c))));;
 
 
 end;;
@@ -604,12 +621,13 @@ let rec focus_to_leaves
 
 let rec wf_fts_trans
   s1 s2 =
-    List.equal_lista
-      (List.equal_list
-        (Product_Type.equal_prod Key_value_types.equal_key
-          Key_value_types.equal_value_t))
-      (focus_to_leaves (Product_Type.fst s2))
-      (focus_to_leaves (Product_Type.fst s1));;
+    Util.assert_true (s1, s2)
+      (List.equal_lista
+        (List.equal_list
+          (Product_Type.equal_prod Key_value_types.equal_key
+            Key_value_types.equal_value_t))
+        (focus_to_leaves (Product_Type.fst s2))
+        (focus_to_leaves (Product_Type.fst s1)));;
 
 let rec dest_fts_state
   fts = let (f, _) = fts in
@@ -618,21 +636,24 @@ let rec dest_fts_state
 
 let rec wellformed_fts_focus
   ms f =
-    let t = Util.rev_apply f Tree_stack.f_t in
-    Tree_stack.wf_core (Util.rev_apply t Tree.tree_to_keys) f &&
-      Tree.wellformed_tree ms t;;
+    Util.assert_true (ms, f)
+      (let t = Util.rev_apply f Tree_stack.f_t in
+       Tree_stack.wf_core (Util.rev_apply t Tree.tree_to_keys) f &&
+         Tree.wellformed_tree ms t);;
 
 let rec wellformed_fts_1
-  fts = (match fts with (_, []) -> true
-          | (c, p :: _) ->
-            Tree_stack.equal_core_t_exta Tree.equal_Tree Product_Type.equal_unit
-              (Tree_stack.mk_child p) c);;
+  fts = Util.assert_true fts
+          (match fts with (_, []) -> true
+            | (c, p :: _) ->
+              Tree_stack.equal_core_t_exta Tree.equal_Tree
+                Product_Type.equal_unit (Tree_stack.mk_child p) c);;
 
 let rec wellformed_fts
-  fts = let (f, ts) = fts in
-        let ms = Tree_stack.ts_to_ms ts in
-        Tree_stack.wellformed_ts ts &&
-          (wellformed_fts_focus ms f && wellformed_fts_1 fts);;
+  fts = Util.assert_true fts
+          (let (f, ts) = fts in
+           let ms = Tree_stack.ts_to_ms ts in
+           Tree_stack.wellformed_ts ts &&
+             (wellformed_fts_focus ms f && wellformed_fts_1 fts));;
 
 
 end;;
@@ -642,7 +663,7 @@ module Delete_tree_stack : sig
   type dts_t =
     D_small_leaf of (Key_value_types.key * Key_value_types.value_t) list |
     D_small_node of (Key_value_types.key list * Tree.tree list) |
-    D_updated_subtree of Tree.tree
+    D_updated_subtree of Tree.tree[@@deriving yojson]
   type dts_state_t =
     Dts_down of
       ((Tree.tree, unit) Tree_stack.core_t_ext *
@@ -652,7 +673,7 @@ module Delete_tree_stack : sig
         ((dts_t, unit) Tree_stack.core_t_ext *
           ((Key_value_types.key list * Tree.tree list), unit)
             Tree_stack.core_t_ext list)
-    | Dts_finished of Tree.tree
+    | Dts_finished of Tree.tree[@@deriving yojson]
   val step_dts : dts_state_t -> dts_state_t option
   val mk_dts_state : Key_value_types.key -> Tree.tree -> dts_state_t
   val focus_to_leaves :
@@ -668,7 +689,7 @@ type dir_t = Right | Left;;
 type dts_t =
   D_small_leaf of (Key_value_types.key * Key_value_types.value_t) list |
   D_small_node of (Key_value_types.key list * Tree.tree list) |
-  D_updated_subtree of Tree.tree;;
+  D_updated_subtree of Tree.tree[@@deriving yojson];;
 
 type dts_state_t =
   Dts_down of
@@ -679,7 +700,7 @@ type dts_state_t =
       ((dts_t, unit) Tree_stack.core_t_ext *
         ((Key_value_types.key list * Tree.tree list), unit)
           Tree_stack.core_t_ext list)
-  | Dts_finished of Tree.tree;;
+  | Dts_finished of Tree.tree[@@deriving yojson];;
 
 let rec dest_lista
   xs = (match xs
@@ -924,8 +945,8 @@ let rec step_up
                            Dts_up (node_merge_right k0 p stka (ks, ts)))
                      | Some _ -> Dts_up (node_steal_left k0 p stka (ks, ts)))
                  | Some _ -> Dts_up (node_steal_right k0 p stka (ks, ts)))
-             | D_updated_subtree _ ->
-               let (_, (ts1, (ks1, (t, (ks2, ts2))))) =
+             | D_updated_subtree t ->
+               let (_, (ts1, (ks1, (_, (ks2, ts2))))) =
                  Util.rev_apply p (Tree_stack.nf_to_aux k0) in
                Dts_up
                  (Util.rev_apply p
@@ -983,14 +1004,11 @@ let rec step_dts
 
 let rec dts_to_ms
   stack_empty dts =
-    (match dts
-      with D_small_leaf _ ->
-        Some (if stack_empty then Constants.Small_root_node_or_leaf
-               else Constants.Small_leaf)
-      | D_small_node (_, _) ->
-        Some (if stack_empty then Constants.Small_root_node_or_leaf
-               else Constants.Small_node)
-      | D_updated_subtree _ -> None);;
+    (match stack_empty with true -> Some Constants.Small_root_node_or_leaf
+      | false ->
+        (match dts with D_small_leaf _ -> Some Constants.Small_leaf
+          | D_small_node (_, _) -> Some Constants.Small_node
+          | D_updated_subtree _ -> None));;
 
 let rec mk_dts_state k0 t = Dts_down (Find_tree_stack.mk_fts_state k0 t);;
 
@@ -1002,16 +1020,23 @@ let rec focus_to_leaves
 
 let rec wf_dts_trans
   s1 s2 =
-    (match (s1, s2)
-      with (Dts_down fts, Dts_down a) -> Find_tree_stack.wf_fts_trans fts a
-      | (Dts_down _, Dts_up _) -> true
-      | (Dts_up du, Dts_up dua) ->
-        List.equal_lista
-          (List.equal_list
+    Util.assert_true (s1, s2)
+      (match (s1, s2)
+        with (Dts_down fts, Dts_down a) -> Find_tree_stack.wf_fts_trans fts a
+        | (Dts_down _, Dts_up _) -> true | (Dts_down _, Dts_finished _) -> true
+        | (Dts_up du, Dts_up dua) ->
+          List.equal_lista
             (Product_Type.equal_prod Key_value_types.equal_key
-              Key_value_types.equal_value_t))
-          (focus_to_leaves (Product_Type.fst dua))
-          (focus_to_leaves (Product_Type.fst du)));;
+              Key_value_types.equal_value_t)
+            (Util.rev_apply (focus_to_leaves (Product_Type.fst dua))
+              List.concat)
+            (Util.rev_apply (focus_to_leaves (Product_Type.fst du)) List.concat)
+        | (Dts_up du, Dts_finished t) ->
+          List.equal_lista
+            (List.equal_list
+              (Product_Type.equal_prod Key_value_types.equal_key
+                Key_value_types.equal_value_t))
+            (focus_to_leaves (Product_Type.fst du)) (Tree.tree_to_leaves t));;
 
 let rec dest_dts_state
   s = (match s with Dts_down _ -> None | Dts_up _ -> None
@@ -1019,40 +1044,49 @@ let rec dest_dts_state
 
 let rec wellformed_dts
   stack_empty dts =
-    let t = Util.rev_apply dts dts_to_tree in
-    let ms = Util.rev_apply dts (dts_to_ms stack_empty) in
-    Tree.wellformed_tree ms t;;
+    Util.assert_true dts
+      (let t = Util.rev_apply dts dts_to_tree in
+       let ms = Util.rev_apply dts (dts_to_ms stack_empty) in
+       Tree.wellformed_tree ms t);;
 
 let rec wellformed_dts_focus
   stack_empty f =
-    let dts = Util.rev_apply f Tree_stack.f_t in
-    Tree_stack.wf_core
-      (Util.rev_apply (Util.rev_apply dts dts_to_tree) Tree.tree_to_keys) f &&
-      wellformed_dts stack_empty dts;;
+    Util.assert_true (stack_empty, f)
+      (let dts = Util.rev_apply f Tree_stack.f_t in
+       Tree_stack.wf_core
+         (Util.rev_apply (Util.rev_apply dts dts_to_tree) Tree.tree_to_keys)
+         f &&
+         wellformed_dts stack_empty dts);;
 
 let rec wellformed_dup_1
-  dup = (match dup with (_, []) -> true
-          | (f, p :: _) ->
-            Tree_stack.equal_core_t_exta Product_Type.equal_unit
-              Product_Type.equal_unit (Util.rev_apply f Tree_stack.without_t)
-              (Util.rev_apply (Tree_stack.mk_child p) Tree_stack.without_t) &&
-              Arith.equal_nat
-                (Util.rev_apply
-                  (Util.rev_apply (Util.rev_apply f Tree_stack.f_t) dts_to_tree)
-                  Tree.height)
-                (Util.rev_apply
-                  (Util.rev_apply (Util.rev_apply p Tree_stack.mk_child)
-                    Tree_stack.f_t)
-                  Tree.height));;
+  dup = Util.assert_true dup
+          (match dup with (_, []) -> true
+            | (f, p :: _) ->
+              Tree_stack.equal_core_t_exta Product_Type.equal_unit
+                Product_Type.equal_unit (Util.rev_apply f Tree_stack.without_t)
+                (Util.rev_apply (Tree_stack.mk_child p) Tree_stack.without_t) &&
+                Arith.equal_nat
+                  (Util.rev_apply
+                    (Util.rev_apply (Util.rev_apply f Tree_stack.f_t)
+                      dts_to_tree)
+                    Tree.height)
+                  (Util.rev_apply
+                    (Util.rev_apply (Util.rev_apply p Tree_stack.mk_child)
+                      Tree_stack.f_t)
+                    Tree.height));;
 
 let rec wellformed_dup
-  dup = let (f, stk) = dup in
-        wellformed_dts_focus (List.null stk) f &&
-          (Tree_stack.wellformed_ts stk && wellformed_dup_1 dup);;
+  dup = Util.assert_true dup
+          (let (f, stk) = dup in
+           wellformed_dts_focus (List.null stk) f &&
+             (Tree_stack.wellformed_ts stk && wellformed_dup_1 dup));;
 
 let rec wellformed_dts_state
-  s = (match s with Dts_down a -> Find_tree_stack.wellformed_fts a
-        | Dts_up (f, stk) -> wellformed_dup (f, stk));;
+  s = Util.assert_true s
+        (match s with Dts_down a -> Find_tree_stack.wellformed_fts a
+          | Dts_up (f, stk) -> wellformed_dup (f, stk)
+          | Dts_finished a ->
+            Tree.wellformed_tree (Some Constants.Small_root_node_or_leaf) a);;
 
 
 end;;
@@ -1060,7 +1094,7 @@ end;;
 
 module Insert_tree_stack : sig
   type its_t = Inserting_one of Tree.tree |
-    Inserting_two of (Tree.tree * (Key_value_types.key * Tree.tree))
+    Inserting_two of (Tree.tree * (Key_value_types.key * Tree.tree))[@@deriving yojson]
   type its_state_t =
     Its_down of
       (((Tree.tree, unit) Tree_stack.core_t_ext *
@@ -1070,7 +1104,7 @@ module Insert_tree_stack : sig
     | Its_up of
         ((its_t, unit) Tree_stack.core_t_ext *
           ((Key_value_types.key list * Tree.tree list), unit)
-            Tree_stack.core_t_ext list)
+            Tree_stack.core_t_ext list)[@@deriving yojson]
   val step_its : its_state_t -> its_state_t option
   val mk_its_state :
     Key_value_types.key -> Key_value_types.value_t -> Tree.tree -> its_state_t
@@ -1083,7 +1117,7 @@ module Insert_tree_stack : sig
 end = struct
 
 type its_t = Inserting_one of Tree.tree |
-  Inserting_two of (Tree.tree * (Key_value_types.key * Tree.tree));;
+  Inserting_two of (Tree.tree * (Key_value_types.key * Tree.tree))[@@deriving yojson];;
 
 type its_state_t =
   Its_down of
@@ -1094,7 +1128,7 @@ type its_state_t =
   | Its_up of
       ((its_t, unit) Tree_stack.core_t_ext *
         ((Key_value_types.key list * Tree.tree list), unit)
-          Tree_stack.core_t_ext list);;
+          Tree_stack.core_t_ext list)[@@deriving yojson];;
 
 let rec split_node
   n = let (ks, ts) = n in
@@ -1195,17 +1229,18 @@ let rec focus_to_leaves
 
 let rec wf_its_trans
   s1 s2 =
-    (match (s1, s2)
-      with (Its_down (fts, v), Its_down (ftsa, va)) ->
-        Find_tree_stack.wf_fts_trans fts ftsa &&
-          Key_value_types.equal_value_ta va v
-      | (Its_down (_, _), Its_up (_, _)) -> true
-      | (Its_up (f, _), Its_up (fa, _)) ->
-        List.equal_lista
-          (List.equal_list
-            (Product_Type.equal_prod Key_value_types.equal_key
-              Key_value_types.equal_value_t))
-          (focus_to_leaves fa) (focus_to_leaves f));;
+    Util.assert_true (s1, s2)
+      (match (s1, s2)
+        with (Its_down (fts, v), Its_down (ftsa, va)) ->
+          Find_tree_stack.wf_fts_trans fts ftsa &&
+            Key_value_types.equal_value_ta va v
+        | (Its_down (_, _), Its_up (_, _)) -> true
+        | (Its_up (f, _), Its_up (fa, _)) ->
+          List.equal_lista
+            (List.equal_list
+              (Product_Type.equal_prod Key_value_types.equal_key
+                Key_value_types.equal_value_t))
+            (focus_to_leaves fa) (focus_to_leaves f));;
 
 let rec dest_its_state
   its = (match its with Its_down _ -> None
@@ -1221,49 +1256,56 @@ let rec dest_its_state
 
 let rec wellformed_its
   stack_empty its =
-    (match its
-      with Inserting_one t ->
-        let ms =
-          (match stack_empty with true -> Some Constants.Small_root_node_or_leaf
-            | false -> None)
-          in
-        Tree.wellformed_tree ms t
-      | Inserting_two (t1, (k, t2)) ->
-        Arith.equal_nat (Tree.height t2) (Tree.height t1) &&
-          (Tree.wellformed_tree None t1 &&
-            (Tree.wellformed_tree None t2 &&
-              (Key_value.check_keys None (Util.rev_apply t1 Tree.tree_to_keys)
-                 (Some k) &&
-                Key_value.check_keys (Some k)
-                  (Util.rev_apply t2 Tree.tree_to_keys) None))));;
+    Util.assert_true (stack_empty, its)
+      (match its
+        with Inserting_one t ->
+          let ms =
+            (match stack_empty
+              with true -> Some Constants.Small_root_node_or_leaf
+              | false -> None)
+            in
+          Tree.wellformed_tree ms t
+        | Inserting_two (t1, (k, t2)) ->
+          Arith.equal_nat (Tree.height t2) (Tree.height t1) &&
+            (Tree.wellformed_tree None t1 &&
+              (Tree.wellformed_tree None t2 &&
+                (Key_value.check_keys None (Util.rev_apply t1 Tree.tree_to_keys)
+                   (Some k) &&
+                  Key_value.check_keys (Some k)
+                    (Util.rev_apply t2 Tree.tree_to_keys) None))));;
 
 let rec wellformed_its_focus
   stack_empty f =
-    let its = Util.rev_apply f Tree_stack.f_t in
-    Tree_stack.wf_core (Util.rev_apply its its_to_keys) f &&
-      wellformed_its stack_empty its;;
+    Util.assert_true (stack_empty, f)
+      (let its = Util.rev_apply f Tree_stack.f_t in
+       Tree_stack.wf_core (Util.rev_apply its its_to_keys) f &&
+         wellformed_its stack_empty its);;
 
 let rec wellformed_iup_1
-  iu = (match iu with (_, []) -> true
-         | (f, p :: _) ->
-           Tree_stack.equal_core_t_exta Product_Type.equal_unit
-             Product_Type.equal_unit (Util.rev_apply f Tree_stack.without_t)
-             (Util.rev_apply (Tree_stack.mk_child p) Tree_stack.without_t) &&
-             Arith.equal_nat
-               (Util.rev_apply (Util.rev_apply f Tree_stack.f_t) its_to_h)
-               (Util.rev_apply
-                 (Util.rev_apply (Util.rev_apply p Tree_stack.mk_child)
-                   Tree_stack.f_t)
-                 Tree.height));;
+  iu = Util.assert_true iu
+         (match iu with (_, []) -> true
+           | (f, p :: _) ->
+             Tree_stack.equal_core_t_exta Product_Type.equal_unit
+               Product_Type.equal_unit (Util.rev_apply f Tree_stack.without_t)
+               (Util.rev_apply (Tree_stack.mk_child p) Tree_stack.without_t) &&
+               Arith.equal_nat
+                 (Util.rev_apply (Util.rev_apply f Tree_stack.f_t) its_to_h)
+                 (Util.rev_apply
+                   (Util.rev_apply (Util.rev_apply p Tree_stack.mk_child)
+                     Tree_stack.f_t)
+                   Tree.height));;
 
 let rec wellformed_iup
-  iu = let (f, stk) = iu in
-       wellformed_its_focus (List.null stk) f &&
-         (Tree_stack.wellformed_ts stk && wellformed_iup_1 iu);;
+  iu = Util.assert_true iu
+         (let (f, stk) = iu in
+          wellformed_its_focus (List.null stk) f &&
+            (Tree_stack.wellformed_ts stk && wellformed_iup_1 iu));;
 
 let rec wellformed_its_state
-  its = (match its with Its_down (fts, _) -> Find_tree_stack.wellformed_fts fts
-          | Its_up (f, stk) -> wellformed_iup (f, stk));;
+  its = Util.assert_true its
+          (match its
+            with Its_down (fts, _) -> Find_tree_stack.wellformed_fts fts
+            | Its_up (f, stk) -> wellformed_iup (f, stk));;
 
 
 end;;
