src/Util.thy
@@ -37,6 +37,10 @@ primrec dest_Some (* :: "'a option => 'a" *) where
 definition is_None :: "'a option \<Rightarrow> bool" where 
 "is_None x == x = None"
   
+(* for debugging ocaml code; otherwise remove *)
+definition assert_true :: "'a \<Rightarrow> bool \<Rightarrow> bool" where
+"assert_true arg b = b"
+
 
 (* rresult -------------------------------------- *)  
   
